wpsim -> wsim

theories/simulations/wsim/wsim.v
@@ -4,27 +4,27 @@ Require Import ISim SMod SMod2HMod HMod.
 
 From stdpp Require Import coPset.
 
-Definition wpsim_ginv (u : univ_id) (n : level) (E : coPset)
+Definition wsim_ginv (u : univ_id) (n : level) (E : coPset)
     `{!invG α Σ Γ, !subG Γ Σ, !sinvG Σ Γ α β τ} : iProp Σ :=
   own_admin ∗ univs u n ∗ wsats u n E.
 
-Lemma wpsim_ginv_split (υ ν : univ_id) (n : level) (E : coPset)
+Lemma wsim_ginv_split (υ ν : univ_id) (n : level) (E : coPset)
     `{!invG α Σ Γ, !subG Γ Σ, !sinvG Σ Γ α β τ} :
   (ν < υ)%positive →
-  wpsim_ginv υ n E ⊣⊢ wpsim_ginv ν n ⊤ ∗ (wpsim_ginv ν n ⊤ -∗ wpsim_ginv υ n E).
+  wsim_ginv υ n E ⊣⊢ wsim_ginv ν n ⊤ ∗ (wsim_ginv ν n ⊤ -∗ wsim_ginv υ n E).
 Proof.
   intros H; iSplit; last (iIntros "[H1 H2]"; iApply ("H2" with "H1")).
   iIntros "[H1 [H2 H3]]".
   iDestruct (univs_split ν υ with "H2") as "[U1 [W1 U2]]"; first done.
   iDestruct (own_admin_split with "H1") as "[O1 O2]".
-  iSplitL "U1 W1 O1"; first rewrite /wpsim_ginv; iFrame.
+  iSplitL "U1 W1 O1"; first rewrite /wsim_ginv; iFrame.
   iIntros "[_ [U W]]"; iApply ("U2" with "U W").
 Qed.
 
 Class WP `{!invG α Σ Γ, !subG Γ Σ, !sinvG Σ Γ α β τ} 
     (P : iProp Σ) (υ : univ_id) (n : level) (E : coPset) := mk_WP {
   WP_remainder : iProp Σ;
-  WP_iff : P ∗-∗ wpsim_ginv υ n E ∗ WP_remainder
+  WP_iff : P ∗-∗ wsim_ginv υ n E ∗ WP_remainder
 }.
 Arguments mk_WP {_ _ _ _ _ _ _ _} _ _ _ _ _ _.
 Arguments WP_remainder {_ _ _ _ _ _ _ _} [_ _ _ _] _.
@@ -36,10 +36,10 @@ Proof. rewrite /ModRel; i; lia. Qed.
 
 Program Global Instance WP_refl `{!invG α Σ Γ, !subG Γ Σ, !sinvG Σ Γ α β τ}
     (υ : univ_id) (n : level) (E : coPset)
-  : WP (wpsim_ginv υ n E) υ n E := mk_WP (wpsim_ginv υ n E) υ n E True _.
+  : WP (wsim_ginv υ n E) υ n E := mk_WP (wsim_ginv υ n E) υ n E True _.
 Next Obligation. ii; iSplit; first iIntros "$"; iIntros "[$ _]". Qed.
 
-Section wpsim.
+Section wsim.
   Context `{!invG α Σ Γ, !subG Γ Σ, !sinvG Σ Γ α β τ}.
 
   Local Definition state : Type := alist key Any.t.
@@ -54,43 +54,43 @@ Section wpsim.
 
   (* TODO : abstraction into mixins *)
   (* TODO : hard-code nodup conditions *)
-  Local Definition wpsim_rel υ n (r : rel) : rel :=
+  Local Definition wsim_rel υ n (r : rel) : rel :=
     λ R_s R_t RR ps pt nths '(st_s, i_s) '(st_t, i_t),
-      (wpsim_ginv υ n ⊤ ∗ r R_s R_t RR ps pt nths (st_s, i_s) (st_t, i_t))%I.
+      (wsim_ginv υ n ⊤ ∗ r R_s R_t RR ps pt nths (st_s, i_s) (st_t, i_t))%I.
 
-  Local Definition wpsim_pre t υ ν n E : iProp Σ :=
+  Local Definition wsim_pre t υ ν n E : iProp Σ :=
     match t with
     | None => emp
-    | Some false => wpsim_ginv ν n ⊤ -∗ wpsim_ginv υ n E
-    | Some true => wpsim_ginv υ n E
+    | Some false => wsim_ginv ν n ⊤ -∗ wsim_ginv υ n E
+    | Some true => wsim_ginv υ n E
     end.
 
   (* Simulation relation that corresponds to iris' weakest precondition *)
-  Local Definition wpsim_def
+  Local Definition wsim_def
       fl_s fl_t Ist my_tid (t : option bool) υ ν n E r g R_s R_t RR ps pt nths st_s st_t
       : iProp Σ :=
-    wpsim_pre t υ ν n E -∗
-    @isim Σ open fl_s fl_t Ist my_tid (wpsim_rel υ n r) (wpsim_rel υ n g)
+    wsim_pre t υ ν n E -∗
+    @isim Σ open fl_s fl_t Ist my_tid (wsim_rel υ n r) (wsim_rel υ n g)
       R_s R_t RR ps pt nths st_s st_t.
-  Local Definition wpsim_aux : seal (@wpsim_def). Proof. by eexists. Qed.
-  Definition wpsim := wpsim_aux.(unseal).
-  Local Definition wpsim_eq : @wpsim = @wpsim_def := wpsim_aux.(seal_eq).
-  Local Ltac unseal := rewrite wpsim_eq /wpsim_def.
+  Local Definition wsim_aux : seal (@wsim_def). Proof. by eexists. Qed.
+  Definition wsim := wsim_aux.(unseal).
+  Local Definition wsim_eq : @wsim = @wsim_def := wsim_aux.(seal_eq).
+  Local Ltac unseal := rewrite wsim_eq /wsim_def.
 
-  Definition wp_fspec (υ : univ_id) (n : level) (fsp : fspec) : fspec :=
+  Definition w_fspec (υ : univ_id) (n : level) (fsp : fspec) : fspec :=
     mk_fspec (meta := fsp.(meta))
       (λ tid x varg arg,
-        wpsim_ginv υ n ⊤ ∗ fsp.(precond) tid x varg arg)%I
+        wsim_ginv υ n ⊤ ∗ fsp.(precond) tid x varg arg)%I
       (λ tid x vret ret,
-        wpsim_ginv υ n ⊤ ∗ fsp.(postcond) tid x vret ret)%I.
+        wsim_ginv υ n ⊤ ∗ fsp.(postcond) tid x vret ret)%I.
   
-  Program Global Instance wp_fspec_precond (fsp : fspec) (υ : univ_id) (n : level) tid m arg varg :
-    WP (precond (wp_fspec υ n fsp) tid m arg varg) υ n ⊤ :=
-    mk_WP (precond (wp_fspec υ n fsp) tid m arg varg) υ n ⊤ (precond fsp tid m arg varg) _.
+  Program Global Instance wsim_fspec_precond (fsp : fspec) (υ : univ_id) (n : level) tid m arg varg :
+    WP (precond (w_fspec υ n fsp) tid m arg varg) υ n ⊤ :=
+    mk_WP (precond (w_fspec υ n fsp) tid m arg varg) υ n ⊤ (precond fsp tid m arg varg) _.
   Next Obligation. intros; iSplit; iIntros "[$ $]". Qed.
 
-  Program Global Instance wp_fspec_postcond (fsp : fspec) (υ : univ_id) (n : level) tid m arg varg :
-    WP (postcond (wp_fspec υ n fsp) tid m arg varg) υ n ⊤ :=
+  Program Global Instance wsim_fspec_postcond (fsp : fspec) (υ : univ_id) (n : level) tid m arg varg :
+    WP (postcond (w_fspec υ n fsp) tid m arg varg) υ n ⊤ :=
     {| WP_remainder := (postcond fsp tid m arg varg) |}.
   Next Obligation. intros; iSplit; iIntros "[$ $]". Qed.
 
@@ -108,36 +108,36 @@ Section wpsim.
     Context (st_s st_t : state).
   
     (* Primitive simulation rules *)
-    Lemma wpsim_init sti_s sti_t :
-      wpsim fl_s fl_t Ist my_tid None υ ν n ⊤ ibot ibot R_s R_t RR ps pt nths sti_s sti_t ⊢
+    Lemma wsim_init sti_s sti_t :
+      wsim fl_s fl_t Ist my_tid None υ ν n ⊤ ibot ibot R_s R_t RR ps pt nths sti_s sti_t ⊢
       @isim Σ open fl_s fl_t Ist my_tid ibot ibot R_s R_t RR ps pt nths sti_s sti_t.
     Proof.
       unseal; iIntros "SIM"; ss; iPoseProof ("SIM" with "[]") as "SIM"; first done.
       iPoseProof (isim_mono_knowledge with "SIM") as "SIM".
-      { instantiate (1:=ibot); i; iIntros "H"; rewrite /wpsim_rel /ibot; destruct sti_src, sti_tgt.
+      { instantiate (1:=ibot); i; iIntros "H"; rewrite /wsim_rel /ibot; destruct sti_src, sti_tgt.
         iDestruct "H" as "[_ []]".
       }
-      { instantiate (1:=ibot); i; iIntros "H"; rewrite /wpsim_rel /ibot; destruct sti_src, sti_tgt.
+      { instantiate (1:=ibot); i; iIntros "H"; rewrite /wsim_rel /ibot; destruct sti_src, sti_tgt.
         iDestruct "H" as "[_ []]".
       }
       iFrame.
     Qed.
 
     (* Mostly will not be used *)
-    Lemma wpsim_ret r g rs rt :
+    Lemma wsim_ret r g rs rt :
       RR nths (st_s, rs) (st_t, rt) ⊢
-      wpsim fl_s fl_t Ist my_tid t υ ν n ⊤ r g R_s R_t RR ps pt nths (st_s, Ret rs) (st_t, Ret rt).
+      wsim fl_s fl_t Ist my_tid t υ ν n ⊤ r g R_s R_t RR ps pt nths (st_s, Ret rs) (st_t, Ret rt).
     Proof. unseal; iIntros "RR I". iApply isim_ret. iFrame. Qed.
 
-    Lemma wpsim_call r g E k_s k_t fn arg :
+    Lemma wsim_call r g E k_s k_t fn arg :
       Ist nths st_s st_t ∗
       (∀ ret nths' st_s' st_t'
         (NODS : List.NoDup (List.map fst st_s'))
         (NODD : List.NoDup (List.map fst st_t')),
         Ist nths' st_s' st_t' -∗
-        wpsim fl_s fl_t Ist my_tid t υ ν n E r g R_s R_t RR true true nths'
+        wsim fl_s fl_t Ist my_tid t υ ν n E r g R_s R_t RR true true nths'
           (st_s', k_s ret) (st_t', k_t ret)) ⊢
-      wpsim fl_s fl_t Ist my_tid t υ ν n E r g R_s R_t RR ps pt nths
+      wsim fl_s fl_t Ist my_tid t υ ν n E r g R_s R_t RR ps pt nths
         (st_s, trigger (Call fn arg) >>= k_s) (st_t, trigger (Call fn arg) >>= k_t).
     Proof.
       unseal; iIntros "[IST CONT] I".
@@ -145,158 +145,158 @@ Section wpsim.
       iIntros (??????) "IST"; iApply ("CONT" with "[] [] [IST]"); iFrame; try iPureIntro; ss.
     Qed.
 
-    Lemma wpsim_io r g fn I O (arg : I) k_s k_t E :
+    Lemma wsim_io r g fn I O (arg : I) k_s k_t E :
       (∀ (ret : O),
-        wpsim fl_s fl_t Ist my_tid t υ ν n E r g R_s R_t RR true true nths
+        wsim fl_s fl_t Ist my_tid t υ ν n E r g R_s R_t RR true true nths
           (st_s, k_s ret) (st_t, k_t ret)) ⊢
-      wpsim fl_s fl_t Ist my_tid t υ ν n E r g R_s R_t RR ps pt nths
+      wsim fl_s fl_t Ist my_tid t υ ν n E r g R_s R_t RR ps pt nths
         (st_s, trigger (IO fn arg) >>= k_s)
         (st_t, trigger (IO fn arg) >>= k_t).
     Proof. unseal; iIntros "RR I". iApply isim_io. iIntros (ret); iApply "RR"; iFrame. Qed.
 
-    Lemma wpsim_tau_src r g i_s i_t E :
-      wpsim fl_s fl_t Ist my_tid t υ ν n E r g R_s R_t RR true pt nths (st_s, i_s) (st_t, i_t) ⊢
-      wpsim fl_s fl_t Ist my_tid t υ ν n E r g R_s R_t RR ps pt nths (st_s, tau;; i_s) (st_t, i_t).
+    Lemma wsim_tau_src r g i_s i_t E :
+      wsim fl_s fl_t Ist my_tid t υ ν n E r g R_s R_t RR true pt nths (st_s, i_s) (st_t, i_t) ⊢
+      wsim fl_s fl_t Ist my_tid t υ ν n E r g R_s R_t RR ps pt nths (st_s, tau;; i_s) (st_t, i_t).
     Proof. unseal; iIntros "RR I". iApply isim_tau_src; iApply "RR"; iFrame. Qed.
 
-    Lemma wpsim_tau_tgt r g i_s i_t E :
-      wpsim fl_s fl_t Ist my_tid t υ ν n E r g R_s R_t RR ps true nths (st_s, i_s) (st_t, i_t) ⊢
-      wpsim fl_s fl_t Ist my_tid t υ ν n E r g R_s R_t RR ps pt nths (st_s, i_s) (st_t, tau;; i_t).
+    Lemma wsim_tau_tgt r g i_s i_t E :
+      wsim fl_s fl_t Ist my_tid t υ ν n E r g R_s R_t RR ps true nths (st_s, i_s) (st_t, i_t) ⊢
+      wsim fl_s fl_t Ist my_tid t υ ν n E r g R_s R_t RR ps pt nths (st_s, i_s) (st_t, tau;; i_t).
     Proof. unseal; iIntros "RR I". iApply isim_tau_tgt; iApply "RR"; iFrame. Qed.
 
-    Lemma wpsim_inline_src r g fn arg f_s k_s i_t E :
+    Lemma wsim_inline_src r g fn arg f_s k_s i_t E :
       alist_find fn fl_s = Some f_s →
-      wpsim fl_s fl_t Ist my_tid t υ ν n E r g R_s R_t RR true pt nths
+      wsim fl_s fl_t Ist my_tid t υ ν n E r g R_s R_t RR true pt nths
         (st_s, x <- (ret <- (f_s arg);; (tau;; tau;; Ret ret));; (k_s x))
         (st_t, i_t) ⊢
-      wpsim fl_s fl_t Ist my_tid t υ ν n E r g R_s R_t RR ps pt nths
+      wsim fl_s fl_t Ist my_tid t υ ν n E r g R_s R_t RR ps pt nths
         (st_s, trigger (Call fn arg) >>= k_s) (st_t, i_t).
     Proof. i; unseal; iIntros "RR I". iApply isim_inline_src; eauto. iApply "RR"; iFrame. Qed.
 
-    Lemma wpsim_inline_tgt r g fn arg i_s f_t k_t E :
+    Lemma wsim_inline_tgt r g fn arg i_s f_t k_t E :
       alist_find fn fl_t = Some f_t →
-      wpsim fl_s fl_t Ist my_tid t υ ν n E r g R_s R_t RR ps true nths
+      wsim fl_s fl_t Ist my_tid t υ ν n E r g R_s R_t RR ps true nths
         (st_s, i_s)
         (st_t, x <- (ret <- (f_t arg);; (tau;; tau;; Ret ret));; (k_t x)) ⊢
-      wpsim fl_s fl_t Ist my_tid t υ ν n E r g R_s R_t RR ps pt nths
+      wsim fl_s fl_t Ist my_tid t υ ν n E r g R_s R_t RR ps pt nths
         (st_s, i_s) (st_t, trigger (Call fn arg) >>= k_t).
     Proof. i; unseal; iIntros "RR I". iApply isim_inline_tgt; eauto. iApply "RR"; iFrame. Qed.
 
-    Lemma wpsim_take_src X r g k_s i_t E :
-      (∀ x, wpsim fl_s fl_t Ist my_tid t υ ν n E r g R_s R_t RR true pt nths
+    Lemma wsim_take_src X r g k_s i_t E :
+      (∀ x, wsim fl_s fl_t Ist my_tid t υ ν n E r g R_s R_t RR true pt nths
         (st_s, k_s x) (st_t, i_t)) ⊢
-      wpsim fl_s fl_t Ist my_tid t υ ν n E r g R_s R_t RR ps pt nths
+      wsim fl_s fl_t Ist my_tid t υ ν n E r g R_s R_t RR ps pt nths
         (st_s, trigger (Take X) >>= k_s) (st_t, i_t).
     Proof.
       unseal; iIntros "RR I". iApply isim_take_src; eauto. iIntros (x); iApply "RR"; iFrame.
     Qed.
 
-    Lemma wpsim_take_tgt X r g i_s k_t E :
+    Lemma wsim_take_tgt X r g i_s k_t E :
       (∃ x,
-        wpsim fl_s fl_t Ist my_tid t υ ν n E r g R_s R_t RR ps true nths (st_s, i_s) (st_t, k_t x)) ⊢
-      wpsim fl_s fl_t Ist my_tid t υ ν n E r g R_s R_t RR ps pt nths
+        wsim fl_s fl_t Ist my_tid t υ ν n E r g R_s R_t RR ps true nths (st_s, i_s) (st_t, k_t x)) ⊢
+      wsim fl_s fl_t Ist my_tid t υ ν n E r g R_s R_t RR ps pt nths
         (st_s, i_s) (st_t, trigger (Take X) >>= k_t).
     Proof.
       unseal; iIntros "[%x RR] I". iApply isim_take_tgt; eauto. iExists _; iApply "RR"; iFrame.
     Qed.
 
-    Lemma wpsim_choose_src X r g k_s i_t E :
+    Lemma wsim_choose_src X r g k_s i_t E :
       (∃ x,
-        wpsim fl_s fl_t Ist my_tid t υ ν n E r g R_s R_t RR true pt nths (st_s, k_s x) (st_t, i_t)) ⊢
-      wpsim fl_s fl_t Ist my_tid t υ ν n E r g R_s R_t RR ps pt nths
+        wsim fl_s fl_t Ist my_tid t υ ν n E r g R_s R_t RR true pt nths (st_s, k_s x) (st_t, i_t)) ⊢
+      wsim fl_s fl_t Ist my_tid t υ ν n E r g R_s R_t RR ps pt nths
         (st_s, trigger (Choose X) >>= k_s) (st_t, i_t).
     Proof.
       unseal; iIntros "[%x RR] I". iApply isim_choose_src; eauto. iExists _; iApply "RR"; iFrame.
     Qed.
 
-    Lemma wpsim_choose_tgt X r g i_s k_t E :
+    Lemma wsim_choose_tgt X r g i_s k_t E :
       (∀ x,
-        wpsim fl_s fl_t Ist my_tid t υ ν n E r g R_s R_t RR ps true nths (st_s, i_s) (st_t, k_t x)) ⊢
-      wpsim fl_s fl_t Ist my_tid t υ ν n E r g R_s R_t RR ps pt nths
+        wsim fl_s fl_t Ist my_tid t υ ν n E r g R_s R_t RR ps true nths (st_s, i_s) (st_t, k_t x)) ⊢
+      wsim fl_s fl_t Ist my_tid t υ ν n E r g R_s R_t RR ps pt nths
         (st_s, i_s) (st_t, trigger (Choose X) >>= k_t).
     Proof.
       unseal; iIntros "RR I". iApply isim_choose_tgt; eauto. iIntros (x); iApply "RR"; iFrame.
     Qed.
 
-    Lemma wpsim_sput_src k v r g k_s i_t E :
-      wpsim fl_s fl_t Ist my_tid t υ ν n E r g R_s R_t RR true pt nths
+    Lemma wsim_sput_src k v r g k_s i_t E :
+      wsim fl_s fl_t Ist my_tid t υ ν n E r g R_s R_t RR true pt nths
         (alist_upd k v st_s, k_s tt) (st_t, i_t) ⊢
-      wpsim fl_s fl_t Ist my_tid t υ ν n E r g R_s R_t RR ps pt nths
+      wsim fl_s fl_t Ist my_tid t υ ν n E r g R_s R_t RR ps pt nths
         (st_s, trigger (SPut k v) >>= k_s) (st_t, i_t).
     Proof. unseal; iIntros "RR I". iApply isim_sput_src; eauto. iApply "RR"; iFrame. Qed.
 
-    Lemma wpsim_sput_tgt k v r g i_s k_t E :
-      wpsim fl_s fl_t Ist my_tid t υ ν n E r g R_s R_t RR ps true nths
+    Lemma wsim_sput_tgt k v r g i_s k_t E :
+      wsim fl_s fl_t Ist my_tid t υ ν n E r g R_s R_t RR ps true nths
         (st_s, i_s) (alist_upd k v st_t, k_t tt) ⊢
-      wpsim fl_s fl_t Ist my_tid t υ ν n E r g R_s R_t RR ps pt nths
+      wsim fl_s fl_t Ist my_tid t υ ν n E r g R_s R_t RR ps pt nths
         (st_s, i_s) (st_t, trigger (SPut k v) >>= k_t).
     Proof. unseal; iIntros "RR I". iApply isim_sput_tgt; eauto. iApply "RR"; iFrame. Qed.
 
-    Lemma wpsim_sget_src k r g k_s i_t E :
-      wpsim fl_s fl_t Ist my_tid t υ ν n E r g R_s R_t RR true pt nths
+    Lemma wsim_sget_src k r g k_s i_t E :
+      wsim fl_s fl_t Ist my_tid t υ ν n E r g R_s R_t RR true pt nths
         (st_s, k_s (or_else (alist_find k st_s) tt↑)) (st_t, i_t) ⊢
-      wpsim fl_s fl_t Ist my_tid t υ ν n E r g R_s R_t RR ps pt nths
+      wsim fl_s fl_t Ist my_tid t υ ν n E r g R_s R_t RR ps pt nths
         (st_s, trigger (SGet k) >>= k_s) (st_t, i_t).
     Proof. unseal; iIntros "RR I". iApply isim_sget_src; eauto. iApply "RR"; iFrame. Qed.
 
-    Lemma wpsim_sget_tgt k r g i_s k_t E :
-      wpsim fl_s fl_t Ist my_tid t υ ν n E r g R_s R_t RR ps true nths
+    Lemma wsim_sget_tgt k r g i_s k_t E :
+      wsim fl_s fl_t Ist my_tid t υ ν n E r g R_s R_t RR ps true nths
         (st_s, i_s) (st_t, k_t (or_else (alist_find k st_t) tt↑)) ⊢
-      wpsim fl_s fl_t Ist my_tid t υ ν n E r g R_s R_t RR ps pt nths
+      wsim fl_s fl_t Ist my_tid t υ ν n E r g R_s R_t RR ps pt nths
         (st_s, i_s) (st_t, trigger (SGet k) >>= k_t).
     Proof. unseal; iIntros "RR I". iApply isim_sget_tgt; eauto. iApply "RR"; iFrame. Qed.
 
-    Lemma wpsim_assume_src (P : iProp Σ) r g k_s i_t E :
-      (P -∗ wpsim fl_s fl_t Ist my_tid t υ ν n E r g R_s R_t RR true pt nths
+    Lemma wsim_assume_src (P : iProp Σ) r g k_s i_t E :
+      (P -∗ wsim fl_s fl_t Ist my_tid t υ ν n E r g R_s R_t RR true pt nths
         (st_s, k_s tt) (st_t, i_t)) ⊢
-      wpsim fl_s fl_t Ist my_tid t υ ν n E r g R_s R_t RR ps pt nths
+      wsim fl_s fl_t Ist my_tid t υ ν n E r g R_s R_t RR ps pt nths
         (st_s, trigger (Assume P) >>= k_s) (st_t, i_t).
     Proof.
       unseal; iIntros "RR I". iApply isim_Assume_src; eauto. iIntros "P".
       iApply ("RR" with "P"); iFrame.
     Qed.
 
-    Lemma wpsim_assume_tgt (P : iProp Σ) r g i_s k_t E :
-      P ∗ wpsim fl_s fl_t Ist my_tid t υ ν n E r g R_s R_t RR ps true nths
+    Lemma wsim_assume_tgt (P : iProp Σ) r g i_s k_t E :
+      P ∗ wsim fl_s fl_t Ist my_tid t υ ν n E r g R_s R_t RR ps true nths
         (st_s, i_s) (st_t, k_t tt) ⊢
-      wpsim fl_s fl_t Ist my_tid t υ ν n E r g R_s R_t RR ps pt nths
+      wsim fl_s fl_t Ist my_tid t υ ν n E r g R_s R_t RR ps pt nths
         (st_s, i_s) (st_t, trigger (Assume P) >>= k_t).
     Proof. unseal; iIntros "[P RR] I". iApply isim_Assume_tgt; eauto. iFrame. iApply "RR". ss. Qed.
 
-    Lemma wpsim_guarantee_src (P : iProp Σ) r g k_s i_t E :
-      P ∗ wpsim fl_s fl_t Ist my_tid t υ ν n E r g R_s R_t RR true pt nths
+    Lemma wsim_guarantee_src (P : iProp Σ) r g k_s i_t E :
+      P ∗ wsim fl_s fl_t Ist my_tid t υ ν n E r g R_s R_t RR true pt nths
         (st_s, k_s tt) (st_t, i_t) ⊢
-      wpsim fl_s fl_t Ist my_tid t υ ν n E r g R_s R_t RR ps pt nths
+      wsim fl_s fl_t Ist my_tid t υ ν n E r g R_s R_t RR ps pt nths
         (st_s, trigger (Guarantee P) >>= k_s) (st_t, i_t).
     Proof.
       unseal; iIntros "[P RR] I". iApply isim_Guarantee_src; eauto. iFrame. iApply "RR"; ss.
     Qed.
 
-    Lemma wpsim_guarantee_tgt (P : iProp Σ) r g i_s k_t E :
-      (P -∗ wpsim fl_s fl_t Ist my_tid t υ ν n E r g R_s R_t RR ps true nths
+    Lemma wsim_guarantee_tgt (P : iProp Σ) r g i_s k_t E :
+      (P -∗ wsim fl_s fl_t Ist my_tid t υ ν n E r g R_s R_t RR ps true nths
         (st_s, i_s) (st_t, k_t tt)) ⊢
-      wpsim fl_s fl_t Ist my_tid t υ ν n E r g R_s R_t RR ps pt nths
+      wsim fl_s fl_t Ist my_tid t υ ν n E r g R_s R_t RR ps pt nths
         (st_s, i_s) (st_t, trigger (Guarantee P) >>= k_t).
     Proof.
       unseal; iIntros "RR I". iApply isim_Guarantee_tgt; eauto.
       iIntros "P"; iApply ("RR" with "P"); done.
     Qed.
 
-    Lemma wpsim_spawn r g fn args k_s k_t E :
-      wpsim fl_s fl_t Ist my_tid t υ ν n E r g R_s R_t RR true true (S nths)
+    Lemma wsim_spawn r g fn args k_s k_t E :
+      wsim fl_s fl_t Ist my_tid t υ ν n E r g R_s R_t RR true true (S nths)
         (st_s, k_s nths) (st_t, k_t nths) ⊢
-      wpsim fl_s fl_t Ist my_tid t υ ν n E r g R_s R_t RR ps pt nths
+      wsim fl_s fl_t Ist my_tid t υ ν n E r g R_s R_t RR ps pt nths
         (st_s, trigger (Spawn fn args) >>= k_s)
         (st_t, trigger (Spawn fn args) >>= k_t).
     Proof. unseal; iIntros "C I". iApply isim_spawn; eauto. iApply "C". ss. Qed.
 
-    Lemma wpsim_yield r g tid k_s k_t E :
+    Lemma wsim_yield r g tid k_s k_t E :
       Ist nths st_s st_t ∗
       (∀ nths' st_s' st_t' (NODS : List.NoDup (map fst st_s')) (NODT : List.NoDup (map fst st_t')),
         Ist nths' st_s' st_t' -∗
-        wpsim fl_s fl_t Ist my_tid t υ ν n E r g R_s R_t RR true true nths'
+        wsim fl_s fl_t Ist my_tid t υ ν n E r g R_s R_t RR true true nths'
           (st_s', k_s tt) (st_t', k_t tt)) ⊢
-      wpsim fl_s fl_t Ist my_tid t υ ν n E r g R_s R_t RR ps pt nths
+      wsim fl_s fl_t Ist my_tid t υ ν n E r g R_s R_t RR ps pt nths
         (st_s, trigger (Yield tid) >>= k_s)
         (st_t, trigger (Yield tid) >>= k_t).
     Proof.
@@ -304,56 +304,56 @@ Section wpsim.
       iIntros (?????) "IST"; iApply ("C" with "[] [] [IST] [I]"); iFrame; iPureIntro; ss.
     Qed.
 
-    Lemma wpsim_tid_src r g k_s i_t E :
-      wpsim fl_s fl_t Ist my_tid t υ ν n E r g R_s R_t RR true pt nths
+    Lemma wsim_tid_src r g k_s i_t E :
+      wsim fl_s fl_t Ist my_tid t υ ν n E r g R_s R_t RR true pt nths
         (st_s, k_s my_tid) (st_t, i_t) ⊢
-      wpsim fl_s fl_t Ist my_tid t υ ν n E r g R_s R_t RR ps pt nths
+      wsim fl_s fl_t Ist my_tid t υ ν n E r g R_s R_t RR ps pt nths
         (st_s, trigger Tid >>= k_s) (st_t, i_t).
     Proof. unseal; iIntros "RR I". iApply isim_tid_src; iApply "RR"; iFrame. Qed.
 
-    Lemma wpsim_tid_tgt r g i_s k_t E :
-      wpsim fl_s fl_t Ist my_tid t υ ν n E r g R_s R_t RR ps true nths
+    Lemma wsim_tid_tgt r g i_s k_t E :
+      wsim fl_s fl_t Ist my_tid t υ ν n E r g R_s R_t RR ps true nths
         (st_s, i_s) (st_t, k_t my_tid) ⊢
-      wpsim fl_s fl_t Ist my_tid t υ ν n E r g R_s R_t RR ps pt nths
+      wsim fl_s fl_t Ist my_tid t υ ν n E r g R_s R_t RR ps pt nths
         (st_s, i_s) (st_t, trigger Tid >>= k_t).
     Proof. unseal; iIntros "RR I". iApply isim_tid_tgt; iApply "RR"; iFrame. Qed.
 
-    Lemma wpsim_reset r g i_s i_t E :
-      wpsim fl_s fl_t Ist my_tid t υ ν n E r g R_s R_t RR false false nths (st_s, i_s) (st_t, i_t) ⊢
-      wpsim fl_s fl_t Ist my_tid t υ ν n E r g R_s R_t RR ps pt nths (st_s, i_s) (st_t, i_t).
+    Lemma wsim_reset r g i_s i_t E :
+      wsim fl_s fl_t Ist my_tid t υ ν n E r g R_s R_t RR false false nths (st_s, i_s) (st_t, i_t) ⊢
+      wsim fl_s fl_t Ist my_tid t υ ν n E r g R_s R_t RR ps pt nths (st_s, i_s) (st_t, i_t).
     Proof. unseal; iIntros "RR I". iApply isim_reset; iApply "RR"; iFrame. Qed.
 
-    Lemma wpsim_progress r g i_s i_t E :
-      wpsim fl_s fl_t Ist my_tid t υ ν n E g g R_s R_t RR false false nths (st_s, i_s) (st_t, i_t) ⊢
-      wpsim fl_s fl_t Ist my_tid t υ ν n E r g R_s R_t RR true true nths (st_s, i_s) (st_t, i_t).
+    Lemma wsim_progress r g i_s i_t E :
+      wsim fl_s fl_t Ist my_tid t υ ν n E g g R_s R_t RR false false nths (st_s, i_s) (st_t, i_t) ⊢
+      wsim fl_s fl_t Ist my_tid t υ ν n E r g R_s R_t RR true true nths (st_s, i_s) (st_t, i_t).
     Proof. unseal; iIntros "RR I". iApply isim_progress; iApply "RR"; iFrame. Qed.
 
-    Lemma wpsim_base r g i_s i_t :
+    Lemma wsim_base r g i_s i_t :
       r R_s R_t RR ps pt nths (st_s, i_s) (st_t, i_t) ⊢
-      wpsim fl_s fl_t Ist my_tid (Some true) υ ν n ⊤ r g R_s R_t RR ps pt nths
+      wsim fl_s fl_t Ist my_tid (Some true) υ ν n ⊤ r g R_s R_t RR ps pt nths
         (st_s, i_s) (st_t, i_t).
     Proof. unseal; iIntros "RR I". iApply isim_base; iFrame. Qed.
 
-    Lemma wpsim_coind (r g : rel) A P RA_s RA_t RRA psA ptA nthsA srcA tgtA :
+    Lemma wsim_coind (r g : rel) A P RA_s RA_t RRA psA ptA nthsA srcA tgtA :
       (∀ (g' : rel) (a : A),
         P a -∗
         (□ ∀ R_s R_t RR ps pt nths0 src tgt,
           g R_s R_t RR ps pt nths0 src tgt -∗ g' R_s R_t RR ps pt nths0 src tgt) -∗
         (□ ∀ a, P a -∗ g' (RA_s a) (RA_t a) (RRA a) (psA a) (ptA a) (nthsA a) (srcA a) (tgtA a)) -∗
-        wpsim fl_s fl_t Ist my_tid (Some true) υ ν n ⊤ r g'
+        wsim fl_s fl_t Ist my_tid (Some true) υ ν n ⊤ r g'
           (RA_s a) (RA_t a) (RRA a) (psA a) (ptA a) (nthsA a) (srcA a) (tgtA a)) →
       ∀ (a : A), P a ⊢
-        wpsim fl_s fl_t Ist my_tid (Some true) υ ν n ⊤ r g
+        wsim fl_s fl_t Ist my_tid (Some true) υ ν n ⊤ r g
           (RA_s a) (RA_t a) (RRA a) (psA a) (ptA a) (nthsA a) (srcA a) (tgtA a).
     Proof.
       unseal; intros H a; iIntros "P I"; iCombine "P I" as "P". iStopProof.
-      (* rewrite /wpsim_retcond *)
+      (* rewrite /wsim_retcond *)
       revert a. eapply isim_coind.
       intros g' a Himpl; iIntros "[[P I] #CIH]".
       iPoseProof (H with "P [] [] I") as "H".
       { instantiate (1 :=
           (λ R_s R_t RR ps pt nths '(st_s, i_s) '(st_t, i_t),
-            wpsim_ginv υ n ⊤ -∗
+            wsim_ginv υ n ⊤ -∗
             g' R_s R_t RR ps pt nths (st_s, i_s) (st_t, i_t))%I).
         iModIntro; iIntros (????????) "G"; destruct src, tgt; iIntros "I". iApply Himpl. iFrame.
       }
@@ -362,17 +362,17 @@ Section wpsim.
       }
       iApply (isim_mono_knowledge with "H"); ss.
       { iIntros (????????) "H"; iModIntro; iFrame. }
-      { iIntros (????????) "H !>"; destruct sti_src, sti_tgt; rewrite /wpsim_rel.
+      { iIntros (????????) "H !>"; destruct sti_src, sti_tgt; rewrite /wsim_rel.
         iDestruct "H" as "[H1 H2]"; iApply "H2"; iFrame.
       }
     Qed.
 
     (* ginv related lemmas *)
-    Lemma wpsim_full_guarantee_src_WP `{i : !WP P υ n E} r g k_s i_t :
+    Lemma wsim_full_guarantee_src_WP `{i : !WP P υ n E} r g k_s i_t :
       (WP_remainder i ∗
-      wpsim fl_s fl_t Ist my_tid None υ ν n E r g R_s R_t RR true pt nths
+      wsim fl_s fl_t Ist my_tid None υ ν n E r g R_s R_t RR true pt nths
         (st_s, k_s tt) (st_t, i_t)) ⊢
-      wpsim fl_s fl_t Ist my_tid (Some true) υ ν n E r g R_s R_t RR ps pt nths
+      wsim fl_s fl_t Ist my_tid (Some true) υ ν n E r g R_s R_t RR ps pt nths
         (st_s, trigger (Guarantee P) >>= k_s) (st_t, i_t).
     Proof.
       unseal; iIntros "[P SIM] I". iApply isim_Guarantee_src; eauto.
@@ -381,21 +381,21 @@ Section wpsim.
       { iApply "SIM"; done. }
     Qed.
 
-    Lemma wpsim_full_guarantee_src (P : iProp Σ) r g k_s i_t E :
-      ((wpsim_ginv υ n E -∗ P) ∗
-      wpsim fl_s fl_t Ist my_tid None υ ν n E r g R_s R_t RR true pt nths
+    Lemma wsim_full_guarantee_src (P : iProp Σ) r g k_s i_t E :
+      ((wsim_ginv υ n E -∗ P) ∗
+      wsim fl_s fl_t Ist my_tid None υ ν n E r g R_s R_t RR true pt nths
         (st_s, k_s tt) (st_t, i_t)) ⊢
-      wpsim fl_s fl_t Ist my_tid (Some true) υ ν n E r g R_s R_t RR ps pt nths
+      wsim fl_s fl_t Ist my_tid (Some true) υ ν n E r g R_s R_t RR ps pt nths
         (st_s, trigger (Guarantee P) >>= k_s) (st_t, i_t).
     Proof.
       unseal; iIntros "[P SIM] I". iApply isim_Guarantee_src; eauto.
       iSplitR "SIM"; iFrame. iApply "P"; iFrame. iApply "SIM"; done.
     Qed.
 
-    Lemma wpsim_full_assume_src_WP `{i : !WP P υ n E} r g k_s i_t :
-      (WP_remainder i -∗ wpsim fl_s fl_t Ist my_tid (Some true) υ ν n E r g R_s R_t RR true pt nths
+    Lemma wsim_full_assume_src_WP `{i : !WP P υ n E} r g k_s i_t :
+      (WP_remainder i -∗ wsim fl_s fl_t Ist my_tid (Some true) υ ν n E r g R_s R_t RR true pt nths
         (st_s, k_s tt) (st_t, i_t)) ⊢
-      wpsim fl_s fl_t Ist my_tid None υ ν n E r g R_s R_t RR ps pt nths
+      wsim fl_s fl_t Ist my_tid None υ ν n E r g R_s R_t RR ps pt nths
         (st_s, trigger (Assume P) >>= k_s) (st_t, i_t).
     Proof.
       unseal; iIntros "SIM _". iApply isim_Assume_src; eauto.
@@ -403,11 +403,11 @@ Section wpsim.
       iApply ("SIM" with "Q I").
     Qed.
 
-    Lemma wpsim_full_assume_src (P P' : iProp Σ) r g k_s i_t E :
-      ((P -∗ (wpsim_ginv υ n E ∗ P')) ∗
-      (P' -∗ wpsim fl_s fl_t Ist my_tid (Some true) υ ν n E r g R_s R_t RR true pt nths
+    Lemma wsim_full_assume_src (P P' : iProp Σ) r g k_s i_t E :
+      ((P -∗ (wsim_ginv υ n E ∗ P')) ∗
+      (P' -∗ wsim fl_s fl_t Ist my_tid (Some true) υ ν n E r g R_s R_t RR true pt nths
         (st_s, k_s tt) (st_t, i_t))) ⊢
-      wpsim fl_s fl_t Ist my_tid None υ ν n E r g R_s R_t RR ps pt nths
+      wsim fl_s fl_t Ist my_tid None υ ν n E r g R_s R_t RR ps pt nths
         (st_s, trigger (Assume P) >>= k_s) (st_t, i_t).
     Proof.
       unseal; iIntros "[P SIM] I". iApply isim_Assume_src; eauto.
@@ -415,14 +415,14 @@ Section wpsim.
       iApply ("SIM" with "P GINV").
     Qed.
 
-    Lemma wpsim_half_assume_tgt_WP `{i : !WP P ν n ⊤, ModRel υ ν} r g i_s k_t E :
+    Lemma wsim_half_assume_tgt_WP `{i : !WP P ν n ⊤, ModRel υ ν} r g i_s k_t E :
       (WP_remainder i ∗
-      wpsim fl_s fl_t Ist my_tid (Some false) υ ν n E r g R_s R_t RR ps true nths
+      wsim fl_s fl_t Ist my_tid (Some false) υ ν n E r g R_s R_t RR ps true nths
         (st_s, i_s) (st_t, k_t tt)) ⊢
-      wpsim fl_s fl_t Ist my_tid (Some true) υ ν n E r g R_s R_t RR ps pt nths
+      wsim fl_s fl_t Ist my_tid (Some true) υ ν n E r g R_s R_t RR ps pt nths
         (st_s, i_s) (st_t, trigger (Assume P) >>= k_t).
     Proof.
-      unseal; iIntros "[P SIM] I". iPoseProof (wpsim_ginv_split with "I") as "[I1 I2]".
+      unseal; iIntros "[P SIM] I". iPoseProof (wsim_ginv_split with "I") as "[I1 I2]".
       { apply H. }
       iApply isim_Assume_tgt; eauto.
       iSplitL "P I1".
@@ -430,24 +430,24 @@ Section wpsim.
       { iApply "SIM"; iFrame. }
     Qed.
 
-    Lemma wpsim_half_guarantee_tgt_WP `{i : !WP P ν n ⊤, ModRel υ ν} r g i_s k_t E :
+    Lemma wsim_half_guarantee_tgt_WP `{i : !WP P ν n ⊤, ModRel υ ν} r g i_s k_t E :
       (WP_remainder i -∗
-      wpsim fl_s fl_t Ist my_tid (Some true) υ ν n E r g R_s R_t RR ps true nths
+      wsim fl_s fl_t Ist my_tid (Some true) υ ν n E r g R_s R_t RR ps true nths
         (st_s, i_s) (st_t, k_t tt)) ⊢
-      wpsim fl_s fl_t Ist my_tid (Some false) υ ν n E r g R_s R_t RR ps pt nths
+      wsim fl_s fl_t Ist my_tid (Some false) υ ν n E r g R_s R_t RR ps pt nths
         (st_s, i_s) (st_t, trigger (Guarantee P) >>= k_t).
     Proof.
       unseal; iIntros "SIM I".
       iApply isim_Guarantee_tgt; iIntros "P"; iPoseProof (WP_iff with "P") as "[P1 P2]".
-      iApply ("SIM" with "P2"); rewrite /wpsim_pre; iApply "I"; done.
+      iApply ("SIM" with "P2"); rewrite /wsim_pre; iApply "I"; done.
     Qed.
 
     (* Derived lemmas *)
-    Lemma wpsim_unwrapU_src r g X (x : option X) k_s i_t E :
+    Lemma wsim_unwrapU_src r g X (x : option X) k_s i_t E :
       (∀ x', ⌜x = Some x'⌝ -∗
-      wpsim fl_s fl_t Ist my_tid t υ ν n E r g R_s R_t RR ps pt nths
+      wsim fl_s fl_t Ist my_tid t υ ν n E r g R_s R_t RR ps pt nths
         (st_s, k_s x') (st_t, i_t)) ⊢
-      wpsim fl_s fl_t Ist my_tid t υ ν n E r g R_s R_t RR ps pt nths
+      wsim fl_s fl_t Ist my_tid t υ ν n E r g R_s R_t RR ps pt nths
         (st_s, unwrapU x >>= k_s) (st_t, i_t).
     Proof.
       iIntros "H". unfold unwrapU. destruct x.
@@ -455,24 +455,24 @@ Section wpsim.
       { unseal; iIntros "P". iApply isim_triggerUB_src. }
     Qed.
 
-    Lemma wpsim_unwrapN_src r g X (x : option X) k_s i_t E :
+    Lemma wsim_unwrapN_src r g X (x : option X) k_s i_t E :
       (∃ x', ⌜x = Some x'⌝ ∗
-        wpsim fl_s fl_t Ist my_tid t υ ν n E r g R_s R_t RR ps pt nths
+        wsim fl_s fl_t Ist my_tid t υ ν n E r g R_s R_t RR ps pt nths
           (st_s, k_s x') (st_t, i_t)) ⊢
-      wpsim fl_s fl_t Ist my_tid t υ ν n E r g R_s R_t RR ps pt nths
+      wsim fl_s fl_t Ist my_tid t υ ν n E r g R_s R_t RR ps pt nths
         (st_s, unwrapN x >>= k_s) (st_t, i_t).
     Proof. iIntros "H". iDestruct "H" as (x') "[% H]". subst. hred_l. iApply "H". Qed.
 
-    Lemma wpsim_sput_src_sandbox scopes k v r g k_s i_t E :
+    Lemma wsim_sput_src_sandbox scopes k v r g k_s i_t E :
       In k.1 scopes →
-      wpsim fl_s fl_t Ist my_tid t υ ν n E r g R_s R_t RR true pt nths
+      wsim fl_s fl_t Ist my_tid t υ ν n E r g R_s R_t RR true pt nths
         (alist_upd k v st_s, k_s tt) (st_t, i_t) ⊢
-      wpsim fl_s fl_t Ist my_tid t υ ν n E r g R_s R_t RR ps pt nths
+      wsim fl_s fl_t Ist my_tid t υ ν n E r g R_s R_t RR ps pt nths
         (st_s, HMod.sandbox scopes (trigger (SPut k v)) >>= k_s) (st_t, i_t).
     Proof.
       intros IN; iIntros "SIM".
       rewrite HModSB.transl_put; des_ifs; ss.
-      { iApply wpsim_sput_src; ss. }
+      { iApply wsim_sput_src; ss. }
       { edestruct (existsb_exists (String.eqb k.1) scopes).
         hexploit H0; ss.
         { exists k.1; split; ss. apply String.eqb_refl. }
@@ -480,16 +480,16 @@ Section wpsim.
       }
     Qed.
 
-    Lemma wpsim_sget_src_sandbox scopes k r g k_s i_t E :
+    Lemma wsim_sget_src_sandbox scopes k r g k_s i_t E :
       In k.1 scopes →
-      wpsim fl_s fl_t Ist my_tid t υ ν n E r g R_s R_t RR true pt nths
+      wsim fl_s fl_t Ist my_tid t υ ν n E r g R_s R_t RR true pt nths
         (st_s, k_s (or_else (alist_find k st_s) tt↑)) (st_t, i_t) ⊢
-      wpsim fl_s fl_t Ist my_tid t υ ν n E r g R_s R_t RR ps pt nths
+      wsim fl_s fl_t Ist my_tid t υ ν n E r g R_s R_t RR ps pt nths
         (st_s, HMod.sandbox scopes (trigger (SGet k)) >>= k_s) (st_t, i_t).
     Proof.
       intros IN; iIntros "SIM".
       rewrite HModSB.transl_get; des_ifs; ss.
-      { iApply wpsim_sget_src; ss. }
+      { iApply wsim_sget_src; ss. }
       { edestruct (existsb_exists (String.eqb k.1) scopes).
         hexploit H0; ss.
         { exists k.1; split; ss. apply String.eqb_refl. }
@@ -497,16 +497,16 @@ Section wpsim.
       }
     Qed.
 
-    Lemma wpsim_sput_tgt_sandbox scopes k v r g i_s k_t E :
+    Lemma wsim_sput_tgt_sandbox scopes k v r g i_s k_t E :
       In k.1 scopes →
-      wpsim fl_s fl_t Ist my_tid t υ ν n E r g R_s R_t RR ps true nths
+      wsim fl_s fl_t Ist my_tid t υ ν n E r g R_s R_t RR ps true nths
         (st_s, i_s) (alist_upd k v st_t, k_t tt) ⊢
-      wpsim fl_s fl_t Ist my_tid t υ ν n E r g R_s R_t RR ps pt nths
+      wsim fl_s fl_t Ist my_tid t υ ν n E r g R_s R_t RR ps pt nths
         (st_s, i_s) (st_t, HMod.sandbox scopes (trigger (SPut k v)) >>= k_t).
     Proof.
       intros IN; iIntros "SIM".
       rewrite HModSB.transl_put; des_ifs; ss.
-      { iApply wpsim_sput_tgt; ss. }
+      { iApply wsim_sput_tgt; ss. }
       { edestruct (existsb_exists (String.eqb k.1) scopes).
         hexploit H0; ss.
         { exists k.1; split; ss. apply String.eqb_refl. }
@@ -514,16 +514,16 @@ Section wpsim.
       }
     Qed.
 
-    Lemma wpsim_sget_tgt_sandbox scopes k r g i_s k_t E :
+    Lemma wsim_sget_tgt_sandbox scopes k r g i_s k_t E :
       In k.1 scopes →
-      wpsim fl_s fl_t Ist my_tid t υ ν n E r g R_s R_t RR ps true nths
+      wsim fl_s fl_t Ist my_tid t υ ν n E r g R_s R_t RR ps true nths
         (st_s, i_s) (st_t, k_t (or_else (alist_find k st_t) tt↑)) ⊢
-      wpsim fl_s fl_t Ist my_tid t υ ν n E r g R_s R_t RR ps pt nths
+      wsim fl_s fl_t Ist my_tid t υ ν n E r g R_s R_t RR ps pt nths
         (st_s, i_s) (st_t, HMod.sandbox scopes (trigger (SGet k)) >>= k_t).
     Proof.
       intros IN; iIntros "SIM".
       rewrite HModSB.transl_get; des_ifs; ss.
-      { iApply wpsim_sget_tgt; ss. }
+      { iApply wsim_sget_tgt; ss. }
       { edestruct (existsb_exists (String.eqb k.1) scopes).
         hexploit H0; ss.
         { exists k.1; split; ss. apply String.eqb_refl. }
@@ -531,40 +531,40 @@ Section wpsim.
       }
     Qed.
 
-    Lemma wpsim_asm_src (P : Prop) r g k_s i_t E :
-      (∀ _ : P, (wpsim fl_s fl_t Ist my_tid t υ ν n E r g R_s R_t RR true pt nths
+    Lemma wsim_asm_src (P : Prop) r g k_s i_t E :
+      (∀ _ : P, (wsim fl_s fl_t Ist my_tid t υ ν n E r g R_s R_t RR true pt nths
         (st_s, k_s tt) (st_t, i_t))) ⊢
-      wpsim fl_s fl_t Ist my_tid t υ ν n E r g R_s R_t RR ps pt nths
+      wsim fl_s fl_t Ist my_tid t υ ν n E r g R_s R_t RR ps pt nths
         (st_s, assume P >>= k_s) (st_t, i_t).
     Proof.
       unseal; iIntros "RR I". iApply isim_asm_src; eauto.
       iIntros "%H"; iApply ("RR" $! H with "I"); iFrame.
     Qed.
 
-    Lemma wpsim_asm_tgt (P : Prop) r g i_s k_t E :
+    Lemma wsim_asm_tgt (P : Prop) r g i_s k_t E :
       P →
-      wpsim fl_s fl_t Ist my_tid t υ ν n E r g R_s R_t RR ps true nths
+      wsim fl_s fl_t Ist my_tid t υ ν n E r g R_s R_t RR ps true nths
         (st_s, i_s) (st_t, k_t tt) ⊢
-      wpsim fl_s fl_t Ist my_tid t υ ν n E r g R_s R_t RR ps pt nths
+      wsim fl_s fl_t Ist my_tid t υ ν n E r g R_s R_t RR ps pt nths
         (st_s, i_s) (st_t, assume P >>= k_t).
     Proof.
       intros H; unseal; iIntros "P I". iApply isim_asm_tgt; eauto. iApply ("P" with "I").
     Qed.
 
-    Lemma wpsim_guar_src (P : Prop) r g k_s i_t E :
+    Lemma wsim_guar_src (P : Prop) r g k_s i_t E :
       P →
-      wpsim fl_s fl_t Ist my_tid t υ ν n E r g R_s R_t RR true pt nths
+      wsim fl_s fl_t Ist my_tid t υ ν n E r g R_s R_t RR true pt nths
         (st_s, k_s tt) (st_t, i_t) ⊢
-      wpsim fl_s fl_t Ist my_tid t υ ν n E r g R_s R_t RR ps pt nths
+      wsim fl_s fl_t Ist my_tid t υ ν n E r g R_s R_t RR ps pt nths
         (st_s, guarantee P >>= k_s) (st_t, i_t).
     Proof.
       intros H; unseal; iIntros "P I". iApply isim_guar_src; eauto. iApply ("P" with "I").
     Qed.
 
-    Lemma wpsim_guar_tgt (P : Prop) r g i_s k_t E :
-      (∀ _ : P, wpsim fl_s fl_t Ist my_tid t υ ν n E r g R_s R_t RR ps true nths
+    Lemma wsim_guar_tgt (P : Prop) r g i_s k_t E :
+      (∀ _ : P, wsim fl_s fl_t Ist my_tid t υ ν n E r g R_s R_t RR ps true nths
         (st_s, i_s) (st_t, k_t tt)) ⊢
-      wpsim fl_s fl_t Ist my_tid t υ ν n E r g R_s R_t RR ps pt nths
+      wsim fl_s fl_t Ist my_tid t υ ν n E r g R_s R_t RR ps pt nths
         (st_s, i_s) (st_t, guarantee P >>= k_t).
     Proof.
       unseal; iIntros "RR I". iApply isim_guar_tgt; eauto.
@@ -572,10 +572,10 @@ Section wpsim.
     Qed.
 
     (* Proofmode instances *)
-    Global Instance wpsim_elim_upd r g P p i_s i_t E :
+    Global Instance wsim_elim_upd r g P p i_s i_t E :
       ElimModal True p false ( |==> P)%I P
-        (wpsim fl_s fl_t Ist my_tid t υ ν n E r g R_s R_t RR ps pt nths (st_s, i_s) (st_t, i_t))
-        (wpsim fl_s fl_t Ist my_tid t υ ν n E r g R_s R_t RR ps pt nths (st_s, i_s) (st_t, i_t)).
+        (wsim fl_s fl_t Ist my_tid t υ ν n E r g R_s R_t RR ps pt nths (st_s, i_s) (st_t, i_t))
+        (wsim fl_s fl_t Ist my_tid t υ ν n E r g R_s R_t RR ps pt nths (st_s, i_s) (st_t, i_t)).
     Proof.
       unseal.
       unfold ElimModal. rewrite bi.intuitionistically_if_elim.
@@ -583,4 +583,4 @@ Section wpsim.
       iApply isim_upd. iMod "H0". iModIntro.
       iApply ("H1" with "H0 HPRE").
     Qed.
-End lemmas. End wpsim.
+End lemmas. End wsim.
