theories/simulations/wsim/wsim_tactics.v
@@ -1,96 +1,96 @@
 Require Import CRIS ltac2_lib.
-Require Export wpsim.
+Require Export wsim.
 
 From iris.proofmode Require Import coq_tactics environments.
 (* ● ◓ ○ *)
 Notation "E1 '------------------------------------------------------------------□' E2 '------------------------------------------------------------------∗' st_src st_tgt '------------------------------params------------------------------' ○ n E r g ps pt '-------------------------------wsim-------------------------------' itr_src itr_tgt" :=
-  (environments.envs_entails (Envs E1 E2 _) (wpsim _ _ _ _ None _ _ n E r g _ _ _ ps pt _ (st_src, itr_src) (st_tgt, itr_tgt)))
+  (environments.envs_entails (Envs E1 E2 _) (wsim _ _ _ _ None _ _ n E r g _ _ _ ps pt _ (st_src, itr_src) (st_tgt, itr_tgt)))
     (at level 50, only printing,
       format "E1 '------------------------------------------------------------------□' '//' E2 '------------------------------------------------------------------∗' '//' st_src '//' st_tgt '//' '------------------------------params------------------------------' '//' ○ '/' n '/' E '/' r '/' g '/' ps '/' pt '//' '-------------------------------wsim-------------------------------' '//' itr_src '//' '//' '//' itr_tgt '//'").
 Notation "E1 '------------------------------------------------------------------□' E2 '------------------------------------------------------------------∗' st_src st_tgt '------------------------------params------------------------------' ◓ n E r g ps pt '-------------------------------wsim-------------------------------' itr_src itr_tgt" :=
-  (environments.envs_entails (Envs E1 E2 _) (wpsim _ _ _ _ (Some false) _ _ n E r g _ _ _ ps pt _ (st_src, itr_src) (st_tgt, itr_tgt)))
+  (environments.envs_entails (Envs E1 E2 _) (wsim _ _ _ _ (Some false) _ _ n E r g _ _ _ ps pt _ (st_src, itr_src) (st_tgt, itr_tgt)))
     (at level 50, only printing,
       format "E1 '------------------------------------------------------------------□' '//' E2 '------------------------------------------------------------------∗' '//' st_src '//' st_tgt '//' '------------------------------params------------------------------' '//' ◓ '/' n '/' E '/' r '/' g '/' ps '/' pt '//' '-------------------------------wsim-------------------------------' '//' itr_src '//' '//' '//' itr_tgt '//'").
 Notation "E1 '------------------------------------------------------------------□' E2 '------------------------------------------------------------------∗' st_src st_tgt '------------------------------params------------------------------' ● n E r g ps pt '-------------------------------wsim-------------------------------' itr_src itr_tgt" :=
-  (environments.envs_entails (Envs E1 E2 _) (wpsim _ _ _ _ (Some true) _ _ n E r g _ _ _ ps pt _ (st_src, itr_src) (st_tgt, itr_tgt)))
+  (environments.envs_entails (Envs E1 E2 _) (wsim _ _ _ _ (Some true) _ _ n E r g _ _ _ ps pt _ (st_src, itr_src) (st_tgt, itr_tgt)))
     (at level 50, only printing,
       format "E1 '------------------------------------------------------------------□' '//' E2 '------------------------------------------------------------------∗' '//' st_src '//' st_tgt '//' '------------------------------params------------------------------' '//' ● '/' n '/' E '/' r '/' g '/' ps '/' pt '//' '-------------------------------wsim-------------------------------' '//' itr_src '//' '//' '//' itr_tgt '//'").
 Notation "E1 '------------------------------------------------------------------□' st_src st_tgt '------------------------------params------------------------------' ○ n E r g ps pt '-------------------------------wsim-------------------------------' itr_src itr_tgt" :=
-  (environments.envs_entails (Envs E1 Enil _) (wpsim _ _ _ _ None _ _ n E r g _ _ _ ps pt _ (st_src, itr_src) (st_tgt, itr_tgt)))
+  (environments.envs_entails (Envs E1 Enil _) (wsim _ _ _ _ None _ _ n E r g _ _ _ ps pt _ (st_src, itr_src) (st_tgt, itr_tgt)))
     (at level 50, only printing,
       format "E1 '------------------------------------------------------------------□' '//' st_src '//' st_tgt '//' '------------------------------params------------------------------' '//' ○ '/' n '/' E '/' r '/' g '/' ps '/' pt '//' '-------------------------------wsim-------------------------------' '//' itr_src '//' '//' '//' itr_tgt '//'").
 Notation "E1 '------------------------------------------------------------------□' st_src st_tgt '------------------------------params------------------------------' ◓ n E r g ps pt '-------------------------------wsim-------------------------------' itr_src itr_tgt" :=
-  (environments.envs_entails (Envs E1 Enil _) (wpsim _ _ _ _ (Some false) _ _ n E r g _ _ _ ps pt _ (st_src, itr_src) (st_tgt, itr_tgt)))
+  (environments.envs_entails (Envs E1 Enil _) (wsim _ _ _ _ (Some false) _ _ n E r g _ _ _ ps pt _ (st_src, itr_src) (st_tgt, itr_tgt)))
     (at level 50, only printing,
       format "E1 '------------------------------------------------------------------□' '//' st_src '//' st_tgt '//' '------------------------------params------------------------------' '//' ◓ '/' n '/' E '/' r '/' g '/' ps '/' pt '//' '-------------------------------wsim-------------------------------' '//' itr_src '//' '//' '//' itr_tgt '//'").
 Notation "E1 '------------------------------------------------------------------□' st_src st_tgt '------------------------------params------------------------------' ● n E r g ps pt '-------------------------------wsim-------------------------------' itr_src itr_tgt" :=
-  (environments.envs_entails (Envs E1 Enil _) (wpsim _ _ _ _ (Some true) _ _ n E r g _ _ _ ps pt _ (st_src, itr_src) (st_tgt, itr_tgt)))
+  (environments.envs_entails (Envs E1 Enil _) (wsim _ _ _ _ (Some true) _ _ n E r g _ _ _ ps pt _ (st_src, itr_src) (st_tgt, itr_tgt)))
     (at level 50, only printing,
       format "E1 '------------------------------------------------------------------□' '//' st_src '//' st_tgt '//' '------------------------------params------------------------------' '//' ● '/' n '/' E '/' r '/' g '/' ps '/' pt '//' '-------------------------------wsim-------------------------------' '//' itr_src '//' '//' '//' itr_tgt '//'").
 Notation "E2 '------------------------------------------------------------------∗' st_src st_tgt '------------------------------params------------------------------' ○ n E r g ps pt '-------------------------------wsim-------------------------------' itr_src itr_tgt" :=
-  (environments.envs_entails (Envs Enil E2 _) (wpsim _ _ _ _ None _ _ n E r g _ _ _ ps pt _ (st_src, itr_src) (st_tgt, itr_tgt)))
+  (environments.envs_entails (Envs Enil E2 _) (wsim _ _ _ _ None _ _ n E r g _ _ _ ps pt _ (st_src, itr_src) (st_tgt, itr_tgt)))
     (at level 50, only printing,
       format "E2 '------------------------------------------------------------------∗' '//' st_src '//' st_tgt '//' '------------------------------params------------------------------' '//' ○ '/' n '/' E '/' r '/' g '/' ps '/' pt '//' '-------------------------------wsim-------------------------------' '//' itr_src '//' '//' '//' itr_tgt '//'").
 Notation "E2 '------------------------------------------------------------------∗' st_src st_tgt '------------------------------params------------------------------' ◓ n E r g ps pt '-------------------------------wsim-------------------------------' itr_src itr_tgt" :=
-  (environments.envs_entails (Envs Enil E2 _) (wpsim _ _ _ _ (Some false) _ _ n E r g _ _ _ ps pt _ (st_src, itr_src) (st_tgt, itr_tgt)))
+  (environments.envs_entails (Envs Enil E2 _) (wsim _ _ _ _ (Some false) _ _ n E r g _ _ _ ps pt _ (st_src, itr_src) (st_tgt, itr_tgt)))
     (at level 50, only printing,
       format "E2 '------------------------------------------------------------------∗' '//' st_src '//' st_tgt '//' '------------------------------params------------------------------' '//' ◓ '/' n '/' E '/' r '/' g '/' ps '/' pt '//' '-------------------------------wsim-------------------------------' '//' itr_src '//' '//' '//' itr_tgt '//'").
 Notation "E2 '------------------------------------------------------------------∗' st_src st_tgt '------------------------------params------------------------------' ● n E r g ps pt '-------------------------------wsim-------------------------------' itr_src itr_tgt" :=
-  (environments.envs_entails (Envs Enil E2 _) (wpsim _ _ _ _ (Some true) _ _ n E r g _ _ _ ps pt _ (st_src, itr_src) (st_tgt, itr_tgt)))
+  (environments.envs_entails (Envs Enil E2 _) (wsim _ _ _ _ (Some true) _ _ n E r g _ _ _ ps pt _ (st_src, itr_src) (st_tgt, itr_tgt)))
     (at level 50, only printing,
       format "E2 '------------------------------------------------------------------∗' '//' st_src '//' st_tgt '//' '------------------------------params------------------------------' '//' ● '/' n '/' E '/' r '/' g '/' ps '/' pt '//' '-------------------------------wsim-------------------------------' '//' itr_src '//' '//' '//' itr_tgt '//'").
 
 (* additional *) 
 Notation "E1 '------------------------------------------------------------------□' E2 '------------------------------------------------------------------∗' st_src st_tgt '-------------------------------wsim-------------------------------' P '∗' 'WSIM'" :=
-  (environments.envs_entails (Envs E1 E2 _) (bi_sep P (wpsim _ _ _ _ _ _ _ _ _ _ _ _ _ _ _ _ _ (st_src, _) (st_tgt, _))))
+  (environments.envs_entails (Envs E1 E2 _) (bi_sep P (wsim _ _ _ _ _ _ _ _ _ _ _ _ _ _ _ _ _ (st_src, _) (st_tgt, _))))
     (at level 50, only printing,
       format "E1 '------------------------------------------------------------------□' '//' E2 '------------------------------------------------------------------∗' '//' st_src '//' st_tgt '//' '-------------------------------wsim-------------------------------' '//' P  '∗'  'WSIM' ").
 
 Notation "E1 '------------------------------------------------------------------□' E2 '------------------------------------------------------------------∗' st_src st_tgt '-------------------------------wsim-------------------------------' P '-∗' 'WSIM'" :=
-  (environments.envs_entails (Envs E1 E2 _) (bi_wand P (wpsim _ _ _ _ _ _ _ _ _ _ _ _ _ _ _ _ _ (st_src, _) (st_tgt, _))))
+  (environments.envs_entails (Envs E1 E2 _) (bi_wand P (wsim _ _ _ _ _ _ _ _ _ _ _ _ _ _ _ _ _ (st_src, _) (st_tgt, _))))
     (at level 50, only printing,
       format "E1 '------------------------------------------------------------------□' '//' E2 '------------------------------------------------------------------∗' '//' st_src '//' st_tgt '//' '-------------------------------wsim-------------------------------' '//' P  '-∗'  'WSIM' ").
 
 Ltac _w_step :=
   match goal with
-  | [ |- environments.envs_entails _ (wpsim _ _ _ _ _ _ _ _ _ _ _ _ _ _ _ _ _ (_, Ret _) (_, Ret _))] =>
-      iApply wpsim_ret
-  | [ |- environments.envs_entails _ (wpsim _ _ _ _ _ _ _ _ _ _ _ _ _ _ _ _ _ (_, trigger (IO _ _) >>= _) (_, trigger (IO _ _) >>= _))] =>
-      iApply wpsim_io; iIntros "%"
-  | [ |- environments.envs_entails _ (wpsim _ _ _ _ _ _ _ _ _ _ _ _ _ _ _ _ _ (_, trigger (Spawn _ _) >>= _) (_, trigger (Spawn _ _) >>= _))] =>
-      iApply wpsim_spawn
+  | [ |- environments.envs_entails _ (wsim _ _ _ _ _ _ _ _ _ _ _ _ _ _ _ _ _ (_, Ret _) (_, Ret _))] =>
+      iApply wsim_ret
+  | [ |- environments.envs_entails _ (wsim _ _ _ _ _ _ _ _ _ _ _ _ _ _ _ _ _ (_, trigger (IO _ _) >>= _) (_, trigger (IO _ _) >>= _))] =>
+      iApply wsim_io; iIntros "%"
+  | [ |- environments.envs_entails _ (wsim _ _ _ _ _ _ _ _ _ _ _ _ _ _ _ _ _ (_, trigger (Spawn _ _) >>= _) (_, trigger (Spawn _ _) >>= _))] =>
+      iApply wsim_spawn
   end.
 
 Ltac _w_step_l :=
   match goal with
-  | [ |- environments.envs_entails _ (wpsim _ _ _ _ _ _ _ _ _ _ _ _ _ _ _ _ _ (_, tau;; _) _) ] =>
-      iApply wpsim_tau_src
-  | [ |- environments.envs_entails _ (wpsim _ _ _ _ _ _ _ _ _ _ _ _ _ _ _ _ _ (_, Ret _ >>= _) _) ] =>
+  | [ |- environments.envs_entails _ (wsim _ _ _ _ _ _ _ _ _ _ _ _ _ _ _ _ _ (_, tau;; _) _) ] =>
+      iApply wsim_tau_src
+  | [ |- environments.envs_entails _ (wsim _ _ _ _ _ _ _ _ _ _ _ _ _ _ _ _ _ (_, Ret _ >>= _) _) ] =>
       rewrite bind_ret_l
-  | [ |- environments.envs_entails _ (wpsim _ _ _ _ _ _ _ _ _ _ _ _ _ _ _ _ _ (_, trigger Tid >>= _) _) ] =>
-      iApply wpsim_tid_src
-  | [ |- environments.envs_entails _ (wpsim _ _ _ _ _ _ _ _ _ _ _ _ _ _ _ _ _ (_, trigger (Take _) >>= _) _) ] =>
-      let name := fresh "q" in iApply wpsim_take_src; iIntros (name)
-  | [ |- environments.envs_entails _ (wpsim _ _ _ _ _ ?υ _ ?n _ _ _ _ _ _ _ _ _ (_, trigger (Assume ?P) >>= _) _) ] =>
+  | [ |- environments.envs_entails _ (wsim _ _ _ _ _ _ _ _ _ _ _ _ _ _ _ _ _ (_, trigger Tid >>= _) _) ] =>
+      iApply wsim_tid_src
+  | [ |- environments.envs_entails _ (wsim _ _ _ _ _ _ _ _ _ _ _ _ _ _ _ _ _ (_, trigger (Take _) >>= _) _) ] =>
+      let name := fresh "q" in iApply wsim_take_src; iIntros (name)
+  | [ |- environments.envs_entails _ (wsim _ _ _ _ _ ?υ _ ?n _ _ _ _ _ _ _ _ _ (_, trigger (Assume ?P) >>= _) _) ] =>
       first [
         tcsearch constr:(WP P υ n ⊤)
           ltac:(fun c =>
-            iApply (wpsim_full_assume_src_WP _ _ _ _ _ _ _ _ _ _ _ _ _ _ _ _ _ _ _ (i:=c)); simpl);
+            iApply (wsim_full_assume_src_WP _ _ _ _ _ _ _ _ _ _ _ _ _ _ _ _ _ _ _ (i:=c)); simpl);
         match goal with
         | [ |- environments.envs_entails _ (?P' -∗ _)] =>
           unfold_precond_postcond P'; iIntrosFresh "ASM"
         end
-      | unfold_precond_postcond P; iApply wpsim_assume_src; iIntrosFresh "ASM"
+      | unfold_precond_postcond P; iApply wsim_assume_src; iIntrosFresh "ASM"
       ]
-  | [ |- environments.envs_entails _ (wpsim _ _ _ _ _ _ _ _ _ _ _ _ _ _ _ _ _ (_, assume _ >>= _) _) ] =>
-      let name := fresh "asm" in iApply wpsim_asm_src; iIntros (name)
-  | [ |- environments.envs_entails _ (wpsim _ _ _ _ _ _ _ _ _ _ _ _ _ _ _ _ _ (_, (HMod.sandbox _ (trigger (SPut _ _))) >>= _) _) ] =>
-      iApply wpsim_sput_src_sandbox; [s;eauto|]
-  | [ |- environments.envs_entails _ (wpsim _ _ _ _ _ _ _ _ _ _ _ _ _ _ _ _ _ (_, (HMod.sandbox _ (trigger (SGet _))) >>= _) _) ] =>
-      iApply wpsim_sget_src_sandbox; [s;eauto|]
-  | [ |- environments.envs_entails _ (wpsim _ _ _ _ _ _ _ _ _ _ _ _ _ _ _ _ _ (_, unwrapU ?ox >>= _) _) ] =>
+  | [ |- environments.envs_entails _ (wsim _ _ _ _ _ _ _ _ _ _ _ _ _ _ _ _ _ (_, assume _ >>= _) _) ] =>
+      let name := fresh "asm" in iApply wsim_asm_src; iIntros (name)
+  | [ |- environments.envs_entails _ (wsim _ _ _ _ _ _ _ _ _ _ _ _ _ _ _ _ _ (_, (HMod.sandbox _ (trigger (SPut _ _))) >>= _) _) ] =>
+      iApply wsim_sput_src_sandbox; [s;eauto|]
+  | [ |- environments.envs_entails _ (wsim _ _ _ _ _ _ _ _ _ _ _ _ _ _ _ _ _ (_, (HMod.sandbox _ (trigger (SGet _))) >>= _) _) ] =>
+      iApply wsim_sget_src_sandbox; [s;eauto|]
+  | [ |- environments.envs_entails _ (wsim _ _ _ _ _ _ _ _ _ _ _ _ _ _ _ _ _ (_, unwrapU ?ox >>= _) _) ] =>
       let name := fresh "q" in
-      iApply wpsim_unwrapU_src; iIntros (name) "%";
+      iApply wsim_unwrapU_src; iIntros (name) "%";
       match goal with [ H: ?x = Some _ |- _ ] => let G := fresh "G" in rename H into G; try rewrite -> G in * end
   end.
 
@@ -127,37 +127,37 @@ Ltac _w_step_r :=
   match goal with
   (******* isim ******)
   (** tgt **)
-  | [ |- environments.envs_entails _ (wpsim _ _ _ _ _ _ _ _ _ _ _ _ _ _ _ _ _ _ (_, tau;; _)) ] =>
-      iApply wpsim_tau_tgt
-  | [ |- environments.envs_entails _ (wpsim _ _ _ _ _ _ _ _ _ _ _ _ _ _ _ _ _ _ (_, Ret _ >>= _) ) ] =>
+  | [ |- environments.envs_entails _ (wsim _ _ _ _ _ _ _ _ _ _ _ _ _ _ _ _ _ _ (_, tau;; _)) ] =>
+      iApply wsim_tau_tgt
+  | [ |- environments.envs_entails _ (wsim _ _ _ _ _ _ _ _ _ _ _ _ _ _ _ _ _ _ (_, Ret _ >>= _) ) ] =>
       rewrite bind_ret_l
-  | [ |- environments.envs_entails _ (wpsim _ _ _ _ _ _ _ _ _ _ _ _ _ _ _ _ _ _ (_, trigger (Choose _) >>= _) ) ] =>
-      let name := fresh "q" in iApply wpsim_choose_tgt; iIntros (name)
-  | [ |- environments.envs_entails _ (wpsim _ _ _ _ _ _ ?ν ?n _ _ _ _ _ _ _ _ _ _ (_, trigger (Guarantee ?P) >>= _) ) ] =>
+  | [ |- environments.envs_entails _ (wsim _ _ _ _ _ _ _ _ _ _ _ _ _ _ _ _ _ _ (_, trigger (Choose _) >>= _) ) ] =>
+      let name := fresh "q" in iApply wsim_choose_tgt; iIntros (name)
+  | [ |- environments.envs_entails _ (wsim _ _ _ _ _ _ ?ν ?n _ _ _ _ _ _ _ _ _ _ (_, trigger (Guarantee ?P) >>= _) ) ] =>
       first [
         tcsearch constr:(WP P ν n ⊤)
           ltac:(fun c =>
-            iApply (wpsim_half_guarantee_tgt_WP _ _ _ _ _ _ _ _ _ _ _ _ _ _ _ _ _ _ _ (i:=c)); simpl);
+            iApply (wsim_half_guarantee_tgt_WP _ _ _ _ _ _ _ _ _ _ _ _ _ _ _ _ _ _ _ (i:=c)); simpl);
         match goal with
         | [ |- environments.envs_entails _ (?P' -∗ _)] =>
           unfold_precond_postcond P'; iIntrosFresh "GRT"
         end
-      | unfold_precond_postcond P; iApply wpsim_guarantee_tgt; iIntrosFresh "GRT"
+      | unfold_precond_postcond P; iApply wsim_guarantee_tgt; iIntrosFresh "GRT"
       ]
-  | [ |- environments.envs_entails _ (wpsim _ _ _ _ _ _ _ _ _ _ _ _ _ _ _ _ _ _ (_, guarantee _ >>= _)) ] =>
-      let name := fresh "grt" in iApply wpsim_guar_tgt; iIntros (name)
-  | [ |- environments.envs_entails _ (wpsim _ _ _ _ _ _ _ _ _ _ _ _ _ _ _ _ _ _ (_, (HMod.sandbox _ (trigger (SPut _ _))) >>= _)) ] =>
-      iApply wpsim_sput_tgt_sandbox; [s; eauto|]
-  | [ |- environments.envs_entails _ (wpsim _ _ _ _ _ _ _ _ _ _ _ _ _ _ _ _ _ _ (_, (HMod.sandbox _ (trigger (SGet _))) >>= _)) ] =>
-      iApply wpsim_sget_tgt_sandbox; [s; eauto|]
+  | [ |- environments.envs_entails _ (wsim _ _ _ _ _ _ _ _ _ _ _ _ _ _ _ _ _ _ (_, guarantee _ >>= _)) ] =>
+      let name := fresh "grt" in iApply wsim_guar_tgt; iIntros (name)
+  | [ |- environments.envs_entails _ (wsim _ _ _ _ _ _ _ _ _ _ _ _ _ _ _ _ _ _ (_, (HMod.sandbox _ (trigger (SPut _ _))) >>= _)) ] =>
+      iApply wsim_sput_tgt_sandbox; [s; eauto|]
+  | [ |- environments.envs_entails _ (wsim _ _ _ _ _ _ _ _ _ _ _ _ _ _ _ _ _ _ (_, (HMod.sandbox _ (trigger (SGet _))) >>= _)) ] =>
+      iApply wsim_sget_tgt_sandbox; [s; eauto|]
   (* 
   | [ |- environments.envs_entails _ (isim _ _ _ _ _ _ _ _ _ _ _ _ (_, unwrapN ?ox >>= _)) ] =>
       let name := fresh "q" in
       iApply isim_unwrapN_tgt; iIntros (name) "%";
       match goal with [ H: ?x = Some _ |- _ ] => let G := fresh "G" in rename H into G; try rewrite -> G in * end
 *)
-  | [ |- environments.envs_entails _ (wpsim _ _ _ _ _ _ _ _ _ _ _ _ _ _ _ _ _ _ (_, trigger Tid >>= _)) ] =>
-      iApply wpsim_tid_tgt
+  | [ |- environments.envs_entails _ (wsim _ _ _ _ _ _ _ _ _ _ _ _ _ _ _ _ _ _ (_, trigger Tid >>= _)) ] =>
+      iApply wsim_tid_tgt
   end.
 
 Ltac w_step_r_core :=
@@ -182,21 +182,21 @@ Ltac w_steps_r :=
 
 Ltac _w_force_l :=
   match goal with
-  | [ |- environments.envs_entails _ (wpsim _ _ _ _ _ _ _ _ _ _ _ _ _ _ _ _ _ (_, trigger (Choose ?T) >>= _) _) ] =>
-      iApply wpsim_choose_src
-  | [ |- environments.envs_entails _ (wpsim _ _ _ _ _ ?υ _ ?n _ _ _ _ _ _ _ _ _ (_, trigger (Guarantee ?P) >>= _) _) ] =>
+  | [ |- environments.envs_entails _ (wsim _ _ _ _ _ _ _ _ _ _ _ _ _ _ _ _ _ (_, trigger (Choose ?T) >>= _) _) ] =>
+      iApply wsim_choose_src
+  | [ |- environments.envs_entails _ (wsim _ _ _ _ _ ?υ _ ?n _ _ _ _ _ _ _ _ _ (_, trigger (Guarantee ?P) >>= _) _) ] =>
       first [
         tcsearch constr:(WP P υ n ⊤)
           ltac:(fun c =>
-            iApply (wpsim_full_guarantee_src_WP _ _ _ _ _ _ _ _ _ _ _ _ _ _ _ _ _ _ _ (i:=c)); simpl);
+            iApply (wsim_full_guarantee_src_WP _ _ _ _ _ _ _ _ _ _ _ _ _ _ _ _ _ _ _ (i:=c)); simpl);
         match goal with
         | [ |- environments.envs_entails _ (?P' ∗ _)] =>
           unfold_precond_postcond P'
         end
-      | unfold_precond_postcond P; iApply wpsim_guarantee_src
+      | unfold_precond_postcond P; iApply wsim_guarantee_src
       ]
-  | [ |- environments.envs_entails _ (wpsim _ _ _ _ _ _ _ _ _ _ _ _ _ _ _ _ _ (_, unwrapN _ >>= _) _) ] =>
-      iApply wpsim_unwrapN_src
+  | [ |- environments.envs_entails _ (wsim _ _ _ _ _ _ _ _ _ _ _ _ _ _ _ _ _ (_, unwrapN _ >>= _) _) ] =>
+      iApply wsim_unwrapN_src
   (* | [ |- environments.envs_entails _ (isim _ _ _ _ _ _ _ _ _ _ _ (_, guarantee _ >>= _) _) ] =>
       iApply isim_guar_src *)
   end.
@@ -218,18 +218,18 @@ Tactic Notation "w_force_l" uconstr(p) :=
 
 Ltac _w_force_r :=
   match goal with
-  | [ |- environments.envs_entails _ (wpsim _ _ _ _ _ _ _ _ _ _ _ _ _ _ _ _ _ _ (_, trigger (Take _) >>= _)) ] =>
-      iApply wpsim_take_tgt
-  | [ |- environments.envs_entails _ (wpsim _ _ _ _ _ _ ?ν ?n _ _ _ _ _ _ _ _ _ _ (_, trigger (Assume ?P) >>= _)) ] =>
+  | [ |- environments.envs_entails _ (wsim _ _ _ _ _ _ _ _ _ _ _ _ _ _ _ _ _ _ (_, trigger (Take _) >>= _)) ] =>
+      iApply wsim_take_tgt
+  | [ |- environments.envs_entails _ (wsim _ _ _ _ _ _ ?ν ?n _ _ _ _ _ _ _ _ _ _ (_, trigger (Assume ?P) >>= _)) ] =>
       first [
         tcsearch constr:(WP P ν n ⊤)
           ltac:(fun c =>
-            iApply (wpsim_half_assume_tgt_WP _ _ _ _ _ _ _ _ _ _ _ _ _ _ _ _ _ _ _ (i:=c)); simpl);
+            iApply (wsim_half_assume_tgt_WP _ _ _ _ _ _ _ _ _ _ _ _ _ _ _ _ _ _ _ (i:=c)); simpl);
         match goal with
         | [ |- environments.envs_entails _ (?P' ∗ _)] =>
           unfold_precond_postcond P'
         end
-      | unfold_precond_postcond P; iApply wpsim_assume_tgt
+      | unfold_precond_postcond P; iApply wsim_assume_tgt
       ]
   (* | [ |- environments.envs_entails _ (isim _ _ _ _ _ _ _ _ _ _ _ _ (_, unwrapU _ >>= _)) ] =>
       iApply isim_unwrapU_tgt; iExists _
@@ -259,7 +259,7 @@ Ltac w_inline_l :=
   hide_ihyps;
   hide_itree_r;
   prep;
-  iApply wpsim_inline_src; [prove_inline_cond|];
+  iApply wsim_inline_src; [prove_inline_cond|];
   unfold_cris_defs;
   show_until marker.
 
@@ -269,12 +269,12 @@ Ltac w_inline_r :=
   hide_ihyps;
   hide_itree_l;
   prep;
-  iApply wpsim_inline_tgt; [prove_inline_cond|];
+  iApply wsim_inline_tgt; [prove_inline_cond|];
   unfold_cris_defs;
   show_until marker.
 
 Ltac by_coind CIH :=
-  iApply wpsim_progress; iApply wpsim_base;
+  iApply wsim_progress; iApply wsim_base;
   iSpecialize (CIH $! _);
   (hrepeat do 1 first[instantiate (1:= (_,_))|instantiate (1:= existT _ _)]); s; grind;
   iApply CIH.
@@ -285,7 +285,7 @@ Ltac w_call hyps :=
   hide_ihyps;
   hide_itree_r; prep; show_itree;
   hide_itree_l; prep; show_itree;
-  iApply wpsim_call;
+  iApply wsim_call;
   show_until marker;
   iSplitL hyps; [try done | iIntros "% % % % % %"; iIntrosFresh "IST"];
   move_aux.
@@ -296,7 +296,7 @@ Ltac yield hyps :=
   hide_ihyps;
   hide_itree_r; prep; show_itree;
   hide_itree_l; prep; show_itree;
-  iApply wpsim_yield
+  iApply wsim_yield
   ; show_until marker
   ; iSplitL hyps; [try done | iIntros "% % % % %"; iIntrosFresh "IST"]
   ; move_aux
@@ -310,8 +310,8 @@ Ltac init_simF :=
   post_simF;
   step_l.
 
-Ltac init_wpsim u_src u_tgt n :=
-  init_simF; iApply (wpsim_init _ _ _ _ u_src u_tgt n).
+Ltac init_wsim u_src u_tgt n :=
+  init_simF; iApply (wsim_init _ _ _ _ u_src u_tgt n).
 
 Ltac unfold_iter_l :=
   let marker := fresh "MARKER" in
